example 1 ready; prod version

WeirdLogic/Example1.lean
@@ -15,17 +15,6 @@ open Unary prim val trm
 open ContextFreeGrammar
 
 
--- -- def SHT_wpmk (label : Set (α ⊕ β)) (i : β) (t : trm) : @SHT (α ⊕ β) :=
--- --   { s := label,
--- --     ht := fun i => [lang|t] }
-
--- /- (fun $i:ident => [lang|$t]) -/
--- syntax "[" num "| " ident " rin " term " => " lang "]" : sht
-
--- macro_rules
---   | `(sht| [$n | $i rin $s => $t]) => `(LGTM.SHT.mk ⟪$n, $s⟫ (fun $i:ident => [lang|$t]))
-
-
 namespace WeirdLogic
 
 def trm1 : trm := [lang| x := x + 1]
@@ -58,22 +47,73 @@ lang_def prog_c1 :=
     else
       x := x + 2
 
-def pay_index : Set (trm ⊕ payload) :=
-  {p:trm ⊕ payload |
-  match p with
-    | Sum.inl _ => False
-    | Sum.inr _ => True
-  }
-def lang_index : Set (trm ⊕ payload ):=
-  {l:trm ⊕ payload |
-    match l with
-    | Sum.inl t => cfg1.Generates (expand_trm t)
-    | Sum.inr _ => False}
+def pay_index' := @Set.univ payload
+abbrev lang := List trm
 
-abbrev pay_index' := @Set.univ payload
+def cfg_expand : Set ( List (Symbol T N)) :=
+  {
+    [Symbol.terminal [lang| x:=x+1]],[Symbol.terminal [lang| x:=x+2]]
+  }
+  -- {
+  --   c | cfg1.Generates c
+  -- }
+
+def pay_index1 : Set payload :=
+  {
+    p | p > 0 ∧ p ∈ pay_index'
+  }
+
+def pay_index2 : Set payload :=
+  {
+    p | p <= 0 ∧ p ∈ pay_index'
+  }
+
+def pay_index : Set (trm × payload) :=
+  {
+    ([lang|()],p) | p ∈ pay_index'
+  }
+
+def lang_list_index' : Set lang :=
+  {l | (trm_to_symbol_list l) ∈ cfg_expand }
 
 def lang_index' : Set trm :=
-  {l | cfg1.Generates (expand_trm l) }
+  {squeeze_trm t | t ∈ lang_list_index'}
+
+def lang_index : Set (trm × payload ):=
+  { (l,0) | l ∈ lang_index' }
+
+lemma lang_unfold :
+  lang_list_index' = {[[lang| x:=x+1]],[[lang| x:=x+2]]} := by
+  unfold lang_list_index' trm_to_symbol_list cfg_expand -- Generates Derives Produces expand_trm
+  ext l
+  simp
+  constructor
+  {
+    intro h
+    induction h with
+    | inl h1 =>
+      left
+      cases l with
+      | nil => simp at h1
+      | cons x xs => simp at h1; unfold trm_to_symbol_list at h1; aesop
+    | inr h2 =>
+      right
+      cases l with
+      | nil => aesop
+      | cons x xs => simp at h2; unfold trm_to_symbol_list at h2; aesop
+  }
+  {
+    intro h
+    induction h with
+    | inl h1=> rw [h1]; aesop
+    | inr h2=> rw [h2]; aesop
+  }
+
+lemma lang_index'_unfold :
+  lang_index' = {[lang| x:=x+1],[lang| x:=x+2]} := by
+  unfold lang_index' squeeze_trm
+  rw [lang_unfold]
+  aesop
 
 def cfg1_left : ContextFreeGrammar trm :=
   {
@@ -95,68 +135,131 @@ def cfg1_right : ContextFreeGrammar trm :=
 
 variable (xptr : loc) (x_ptr : ℤ -> ℤ)
 
-lemma example4_spec_origin(f : ℤ -> val):
-  {
-    [∗ in Set.univ | H ] ∗ arr⟨⋆⟩(xptr , i in 1 =>f i)
-  }
-  [0| p in pay_index => prog_c1(⟨val_int (Sum.getRight! p.val)⟩)]
-  [1| l in lang_index => ⟦Sum.getLeft! l.val⟧]
-  { v,
-    fun h => ∀ l ∈ lang_index', ∃ p , h ⟨1, Sum.inl l⟩ = h ⟨0, Sum.inr p⟩
-  } := by
-  unfold LGTM.triple
-  sorry
+-- lemma example4_spec_origin(f : ℤ -> val):
+--   {
+--     [∗ in Set.univ | H ] ∗ arr⟨⋆⟩(xptr , i in 1 =>f i)
+--   }
+--   [0| p in pay_index => prog_c1(⟨val_int (Sum.getRight! p.val)⟩)]
+--   [1| l in lang_index => ⟦Sum.getLeft! l.val⟧]
+--   { v,
+--     fun h => ∀ l ∈ lang_index', ∃ p , h ⟨1, Sum.inl l⟩ = h ⟨0, Sum.inr p⟩
+--   } := by
+--   unfold LGTM.triple
+--   sorry
 
-lemma example4_spec (f : ℤ -> val):
-  LGTM.triple
-  [{ s := ⟪0, pay_index⟫, ht := fun p ↦ prog_c1.trm_call [(Sum.getRight! p.val)] },
-    { s := ⟪1, lang_index⟫, ht := fun l ↦ (Sum.getLeft! l.val) }]
-  ( [∗ in Set.univ | H ] ∗ arr⟨⋆⟩(xptr , i in 1 =>f i))
-  (fun v => fun h => (∀ l ∈ { ll | Sum.inl l ∈ lang_index}, ∃ p ∈ { pp | Sum.inr pp ∈ pay_index}, h ⟨1, Sum.inl l⟩ = h ⟨0, Sum.inr p⟩))
-  := by
-  unfold LGTM.triple
-  simp_all
-  unfold prog_c1
-  sorry
 
 abbrev default_payload : payload:= 0
 abbrev default_trm : trm := [lang|()]
-
-def pay_idx_prod : Set (trm × payload) :=
-  {
-    ([lang|()],p) | p ∈ @Set.univ payload
-  }
-def lang_set : Set trm :=
-  {l | cfg1.Generates (expand_trm l)}
 
 def lang_set1 : Set trm :=
   {[lang| x := x + 1]}
 def lang_set2 : Set trm :=
   {[lang| x := x + 2]}
-def lang_idx_prod : Set (trm × payload ):=
-  { (l, 0) | l ∈ lang_set}
 
-lemma example4_spec' (f : ℤ -> val):
+lemma arr_union_eq (f : ℤ -> val):
+  s = s₁ ∪ s₂ ->
+  Disjoint s₁ s₂ ->
+  arr⟨s⟩(xptr , i in 1 =>f i) = arr⟨s₁⟩(xptr , i in 1 =>f i) ∗ arr⟨s₂⟩(xptr , i in 1 =>f i) := by
+  move=> unio disj
+  unfold hharrayFun
+  rw [unio]
+  apply eq_comm.mpr
+  apply bighstar_hhstar_disj=>//
+
+lemma example4_spec (f : ℤ -> val):
   {
     -- [∗ in Set.univ | H ] ∗
-    arr⟨⋆⟩(xptr , i in 1 =>f i)
+    arr⟨{⟨0,p⟩ | p ∈ pay_index}⟩(xptr , i in 1 =>f i) ∗
+    arr⟨{⟨1,l⟩ | l ∈ lang_index}⟩(xptr , i in 1 =>f i)
   }
-  [0| p in pay_idx_prod => prog_c1(⸨xptr: Loc⸩, ⟨p.val.2⟩)]
-  [1| l in lang_idx_prod => ⟦l.val.1⟧]
+  [0| p in pay_index => prog_c1(⸨xptr: Loc⸩, ⟨p.val.2⟩)]
+  [1| l in lang_index => ⟦l.val.1⟧]
   { v,
-    fun h => ∀ l ∈ lang_idx_prod, ∃ p ∈ pay_idx_prod , h ⟨1, l⟩ = h ⟨0, p⟩
+    fun h => ∀ l ∈ lang_index, ∃ p ∈ pay_index , h ⟨1, l⟩ = h ⟨0, p⟩
   }
   := by
   unfold LGTM.triple
-  apply weird_grmdisj_lemma' (s' := {([lang| x := x + 1],0)}) (s'' := pay_idx_prod) (s := lang_idx_prod)
-    (HH := arr⟨{⟨0,p⟩ | p ∈ pay_idx_prod}⟩(xptr , i in 1 =>f i))
+  rw [hhstar_comm]
+  rw [arr_union_eq (s₁ := {⟨ 1,(l,default_payload)⟩ | l ∈ lang_set1}) (s₂ := {⟨ 1, (l,default_payload)⟩ | l ∈ lang_set2}) ]
+  rotate_left
+  {
+    unfold lang_index default_payload lang_set1 lang_set2
+    rw [lang_index'_unfold]
+    aesop
+  }
+  { apply disjoint_iff.mpr
+    unfold lang_set1 lang_set2
+    aesop
+   }
+  rw [hhstar_comm]
+  apply weird_grmdisj_lemma' (s' := {([lang| x := x + 2],0)}) (s'' := pay_index) (s := lang_index)
+    (HH := arr⟨{⟨0,p⟩ | p ∈ pay_index}⟩(xptr , i in 1 =>f i))
     (H₂ := arr⟨{⟨ 1,(l,default_payload)⟩ | l ∈ lang_set2}⟩(xptr , i in 1 =>f i))
     (H₁ := arr⟨{⟨ 1, (l,default_payload)⟩ | l ∈ lang_set1}⟩(xptr , i in 1 =>f i))=>//
-  · unfold lang_idx_prod lang_set expand_trm; simp; sorry
+  · unfold lang_index
+    rw [lang_index'_unfold]
+    aesop
   · simp; apply disjoint_label_set.mpr; aesop
-  · sorry
   /- left part -/
-  · sorry
+  · rw [arr_union_eq (s₁ := {⟨0,(default_trm,p)⟩ | p ∈ pay_index1}) (s₂ := {⟨0,(default_trm,p)⟩ | p ∈ pay_index2})]
+    rotate_left
+    { unfold pay_index pay_index' pay_index1 pay_index2 default_trm pay_index'
+      simp
+      ext x
+      constructor
+      · intro ⟨a, ha⟩
+        by_cases h : 0 < a
+        · left
+          use a
+        · right
+          use a
+          exact ⟨le_of_not_gt h, ha⟩
+      · intro hx
+        cases hx with
+        | inl h₁ => aesop
+        | inr h₂ => aesop
+        }
+    {
+      apply disjoint_iff.mpr
+      simp
+      unfold pay_index1 pay_index2 pay_index'
+      ext x
+      constructor
+      · intro ⟨⟨p₁, hp₁_mem, hx₁⟩, ⟨p₂, hp₂_mem, hx₂⟩⟩
+        have : p₁ = p₂ := by
+          injection (hx₁.trans hx₂.symm)
+          aesop
+        subst this
+        have hcontr : ¬ (p₁ > 0 ∧ p₁ ≤ 0) := by
+          intro h
+          exact not_lt_of_ge h.2 h.1
+        exact hcontr ⟨hp₁_mem.1, hp₂_mem.1⟩
+      · intro h
+        cases h
+    }
+    rw [hhstar_assoc]
+    apply weird_weaken_lemma' (s' := {(default_trm,p) | p ∈ pay_index1}) (s := pay_index)
+      (H₁ := arr⟨{⟨0,(default_trm,p)⟩ | p ∈ pay_index1}⟩(xptr , i in 1 =>f i))=>//
+    · unfold pay_index1 pay_index' pay_index pay_index'
+      simp
+    · apply disjoint_label_set.mpr; simp
+    · /- part 1: sht_prog only -/
+      unfold pay_index1 pay_index' pay_index pay_index'
+      simp
+      sorry
+    · /- part 2: if-true case -/
+      have simp_lang : lang_index \ {([lang| x := x + 2],0)} = {([lang| x:=x+1],0)} := by
+        unfold lang_index
+        rw [lang_index'_unfold]
+        aesop
+      rw [simp_lang]
+      apply weird_lang_lemma'=>//
+      { simp; apply disjoint_label_set.mpr; aesop }
+      apply weird_payload_lemma' (pr := (default_trm, 10))=>//
+      { simp; apply disjoint_label_set.mpr; aesop }
+      simp
+      -- rw [← weird_fix_lang]
+      sorry
   /- right part -/
   · sorry
 
@@ -164,9 +267,17 @@ lemma example4_spec' (f : ℤ -> val):
 #print bighstar_hhstar_disj
 -- #check ystep
 
-lemma hharray_disj (s₁ s₂ : Set α) (f : ℤ → val):
+lemma hharray_disj (s₁ : Set α) (f : ℤ → val):
   arr⟨s₁⟩(p , x in n =>f x) ∗ arr⟨⋆ \ s₁⟩(p , x in n =>f x) = arr⟨⋆⟩(p , x in n =>f x) :=by
-  sorry
+  have tmp : arr⟨⋆⟩(p , x in n =>f x) = arr⟨s₁ ∪ (⋆ \ s₁)⟩(p , x in n =>f x) := by
+    congr!
+    exact Eq.symm (Set.union_diff_cancel' (fun ⦃a⦄ a ↦ a) fun ⦃a⦄ a ↦ trivial)
+  rw [tmp]
+  unfold hharrayFun
+  apply eq_comm.mpr
+  symm
+  apply bighstar_hhstar_disj (s₂ := ⋆ \ s₁)=>//
+  exact Set.disjoint_sdiff_right
 
 def left_lang_index : Set (trm ⊕ payload):= {l:trm ⊕ payload |
       match l with
@@ -193,8 +304,9 @@ lemma example4_spec_hete (f : ℤ -> val):
   unfold LGTM.triple
   unfold LGTM.HSHT.mkSHT LGTM.Labeled.map Set.image
   dsimp
+  stop
   apply weird_grmdisj_lemma
-    (s' := left_lang_index) (s := lang_index) (s'' := pay_index)
+    (s' := left_lang_index)
     (H := arr⟨⟪0,⋆ ⟫⟩(xptr , i in 1 =>f i))
     (H₁ := arr⟨⟪1,left_lang_index⟫⟩(xptr , i in 1 =>f i))
     (H₂ := arr⟨⟪1,right_lang_index⟫⟩(xptr , i in 1 =>f i))
