WeirdLogic/WLogic.lean
@@ -35,6 +35,22 @@ lemma hheap_weaken_forall (α β: Type) (i j : ℕ) (h : hheap (Labeled (α ⊕ 
   exact hsub
   simp_all only
 
+lemma hheap_exists_superset (h : hheap (Labeled α )) (P P₁: Set α ):
+  P₁ ⊆ P ->
+  (∃ p ∈ P₁, h ⟨j, l⟩ = h ⟨i, p⟩ )->
+  ∃ p ∈ P, h ⟨j, l⟩ = h ⟨i, p⟩ := by
+  move=> sub h1
+  rcases h1 with ⟨p1, hp1, hp2⟩
+  use p1
+  aesop
+
+lemma hheap_weaken_forall' (α : Type) (i j : ℕ) (h : hheap (Labeled α )) (P P₁ L: Set α ) (hsub : P₁ ⊆ P):
+  (∀ ll ∈ L, ∃ p ∈ P₁, h ⟨j, ll ⟩= h ⟨i, p⟩) → ∀ ll ∈ L, ∃ p ∈ P, h ⟨j, ll ⟩= h ⟨i, p⟩ := by
+  intro hle l
+  move=> hl
+  specialize hle l hl
+  aesop
+
 #check Unary.wp_conseq
 
 lemma weird_wp_conseq (t : LGTM.SHTs (Labeled α)) (Q1 Q2 : hval (Labeled α) → hhProp (Labeled α)) :
@@ -64,10 +80,30 @@ lemma weird_weaken_mid_post_lemma (i j : ℕ) (s' s s'': Set (α ⊕ β)) (sht_p
     specialize w h₁
     aesop
 
+lemma weird_weaken_mid_post_lemma' (α : Type) (i j : ℕ) (s' s s'': Set α) (sht_prog sht_lang : LGTM.SHT):
+  sht_prog.s = ⟪i, s⟫ ->
+  sht_lang.s = ⟪ j, s''⟫ ->
+  s' ⊆ s -> Disjoint sht_prog.s sht_lang.s ->
+  LGTM.wp [sht_prog, sht_lang] (fun _ h => ∀ ll ∈ s'', ∃ pp ∈ s', h ⟨j, ll ⟩= h ⟨i, pp⟩)
+  ==> LGTM.wp [sht_prog, sht_lang] (fun _ h => ∀ ll ∈ s'', ∃ pp ∈ s, h ⟨j, ll ⟩= h ⟨i, pp⟩) := by
+  move=> _ _ subst *
+  apply weird_wp_conseq
+  intro x h
+  intro w
+  apply hheap_weaken_forall'=>//
+
+lemma lang_singleton_forall_eq (i j : ℕ) (s s': Set α ) (l : α ) (h : hheap αˡ ):
+  s = {l} ->
+  ∀ ll ∈ s, ∃ pp ∈ s', h ⟨j, ll ⟩= h ⟨i, pp⟩ =
+  ∃ pp ∈ s', h ⟨j, l ⟩= h ⟨i, pp⟩ := by
+  move=>single
+  aesop
+
 #check heval_nonrel
 #print bighstarDef
 #check hhstar
 #print hheap
+#check Set.mem_singleton_iff
 
 lemma weird_heap_sub_left (i j : ℕ) (Q : hhProp (α ⊕ β)ˡ) (s s' s'': Set (α ⊕ β)) :
   i ≠ j ->
@@ -124,6 +160,32 @@ lemma weird_heap_sub_right (i j : ℕ) (Q : hhProp (α ⊕ β)ˡ) (s s' s'': Set
     aesop
   · aesop
 
+lemma weird_heap_sub_right' (i j : ℕ) (Q : hhProp αˡ) (s s' s'': Set α) :
+  i ≠ j ->
+  hhlocal (⟪i, s⟫ \ ⟪i, s'⟫ ) Q ->
+  hhstar (fun h => ∀ ll ∈ {l | l ∈ s''}, ∃ pp,
+     pp ∈ s' ∧ h ⟨j, ll ⟩= h ⟨i, pp⟩) Q
+  ==>
+  (fun h => ∀ ll ∈ {l |  l ∈ s''}, ∃ pp,
+    pp ∈ s' ∧ h ⟨j, ll ⟩= h ⟨i, pp⟩)  := by
+  unfold hhstar hhlocal hlocal
+  intro ij hl
+  move=> hh hs
+  rcases hs with ⟨ hh1, hh2, ⟨ hs1,hs2,hs3, hs4 ⟩ ⟩
+  subst hh
+  simp
+  specialize hl _ hs2
+  intro ll lin
+  rw [hl]
+  · simp at hs1
+    specialize hs1 ll lin
+    rcases hs1 with ⟨pp, hs11, hs12⟩
+    exists pp
+    rw [hl]
+    simp_all
+    simp
+    aesop
+  · aesop
 
 -- #print yfocus_set_lemma
 -- #check qstar
@@ -272,6 +334,7 @@ lemma yfocus_set_lemma_eq (idx : ℕ) (l : LabType) (s' s : Set α) (shts : LGTM
     (hwp ⟪l, s \ s'⟫ shts[idx].ht fun hv =>
     LGTM.wp ((shts.eraseIdx (idx)).insertIdx idx ⟨⟪l, s ∩ s'⟫,shts[idx].ht⟩) fun hv' =>
       Q $ fun_lab_insert l (hv' ∪_⟪l,s'⟫ hv) hv') = LGTM.wp shts Q := by
+    stop -- to save time for testing
     move=> seq --uniset
     move =>/[dup]?/List.pairwise_iff_getElem dj' /[dup] dj₁ /Set.disjoint_left dj
     srw (LGTM.wp_focus idx) //' seq -(Set.diff_union_inter ⟪l,s⟫ ⟪l,s'⟫) /==
@@ -449,6 +512,56 @@ lemma weird_weaken_lemma  (s' s s'': Set (α ⊕ β)) (sht_prog sht_lang : LGTM.
     convert form2
     aesop
 
+/- Prod version: s' is the part to keep (P' in weaken rule) -/
+lemma weird_weaken_lemma' (s' s s'': Set α) (sht_prog sht_lang : LGTM.SHT):
+  sht_prog.s = ⟪0, s⟫ ->
+  sht_lang.s = ⟪1, s''⟫ ->
+  s' ⊆ s -> Disjoint sht_prog.s sht_lang.s ->
+  H₁ ==> LGTM.wp [⟨⟪0, s \ s'⟫, sht_prog.ht⟩] (fun _ => fun h ↦ ∀ a, a ∉ ⟪0, s \ s'⟫ ∧ h a = ∅ ) ->
+  H₂ ==> LGTM.wp [⟨⟪0, s'⟫, sht_prog.ht⟩, sht_lang]
+    (fun _ h => ∀ ll ∈ s'', ∃ pp ∈ s', h ⟨1,ll⟩= h ⟨0, pp⟩ ) ->
+  H₁ ∗ H₂ ==> LGTM.wp [sht_prog, sht_lang]
+  (fun _ h => ∀ ll ∈ s'', ∃ pp ∈ s, h ⟨1, ll ⟩= h ⟨0, pp⟩) := by
+  move=> prog lang subs disj part1 part2
+  intro h12
+  move=> H12
+  apply weird_weaken_mid_post_lemma'=>//
+  set Qp1 : hval αˡ → hhProp αˡ:= fun _ => (fun h ↦ ∀ ll ∈ s'', ∃ pp ∈ s', h ⟨1, ll⟩ = h ⟨0, pp⟩)
+  set B : hhProp αˡ:= fun h ↦ ∀ a, a ∉ ⟪0, s \ s'⟫ ∧ h a = ∅
+  set B' : hval αˡ → hhProp αˡ:= fun _ => B
+  apply weird_wp_conseq (Q1 := whqstar Qp1 B)
+  · unfold whqstar B Qp1
+    intro x
+    simp
+    move=> hc hcon
+    apply weird_heap_sub_right' (s := s) (s'' := s'') (Q := B)=>//
+    · unfold hhlocal hlocal B
+      intro h
+      dsimp
+      aesop
+    · unfold B
+      simp_all
+  apply well_formed_focus_lemma (idx := 0) (l := 0) (shts := [sht_prog, sht_lang]) (s' := s') (s := s) (H := B' ∗ H₂) (R := H₁ ∗ H₂) (Q := Qp1 ∗ B)=>//
+  · simp_all; apply disjoint_label_set.mpr; aesop
+  · have part11 := (hhimpl_frame_l (hH₃ := H₂) (hH₁ := H₁) (hH₂ := LGTM.wp [{ s := ⟪0, s \ s'⟫, ht := sht_prog.ht }] B'))
+    specialize part11 part1
+    simp
+    apply hhimpl_trans (h₁ := H₁ ∗ H₂ ) ( h₂ := ((LGTM.wp [{ s := ⟪0, s \ s'⟫, ht := sht_prog.ht }] B') ∗ H₂)) (h₃ := LGTM.wp [{ s := ⟪0, s \ s'⟫, ht := sht_prog.ht }] (B' ∗ H₂))
+    · exact part11
+    · have form1 := LGTM.wp_frame (Q := B') (H := H₂) (sht := [{ s := ⟪0, s \ s'⟫, ht := sht_prog.ht }])
+      convert form1
+  intro x
+  have part21 := (hhimpl_frame_l (hH₃ := B) (hH₁ := H₂) (hH₂ := LGTM.wp [{ s := ⟪0, s'⟫, ht := sht_prog.ht }, sht_lang] Qp1))
+  specialize part21 part2
+  simp
+  unfold B'
+  rw [hhstar_comm]
+  apply hhimpl_trans (h₁ := H₂ ∗ B) ( h₂ := LGTM.wp [{ s := ⟪0, s'⟫, ht := sht_prog.ht }, sht_lang] Qp1 ∗ B) (h₃ := LGTM.wp [{ s := ⟪0, s ∩ s'⟫, ht := sht_prog.ht }, sht_lang] (Qp1 ∗ B))
+  · exact part21
+  · have form2 := LGTM.wp_frame ( Q := Qp1) (H := B) (sht := [{ s := ⟪0, s'⟫, ht := sht_prog.ht }, sht_lang])
+    convert form2
+    aesop
+
 #check hwp_union
 #check LGTM.wp_cons
 #check eval_conseq
@@ -599,15 +712,27 @@ lemma weird_strengthen_lang (s : Set (α ⊕ β)) (sht_prog sht_lang sht_lang': 
 /- ********************************** GrmDisj Rule ************************************** -/
 
 /- Another format of Grmdisj rule using product type-/
-open AddPCM
-lemma weird_grmdisj_lemma' (s' s : Set (α × β)) (H₃ HH H₁ H₂ : hhProp (α × β)ˡ) (sht_prog sht_lang : LGTM.SHT) :
+
+lemma weird_grmdisj_lemma_aux' (s' s : Set (α × β)) (H₃ HH H₁ H₂ : hhProp (α × β)ˡ) (Q : hval (α × β)ˡ → hhProp (α × β)ˡ) (sht_prog sht_lang : LGTM.SHT) :
+  sht_prog.s = ⟪0, s''⟫ ->
+  sht_lang.s = ⟪ 1, s⟫ ->
+  s' ⊆ s -> Disjoint sht_prog.s sht_lang.s ->
+  HH ∗ H₁ ==> LGTM.wp [sht_prog] (fun hv1 => LGTM.wp [sht_lang1] fun hv2 => Q (hv2 ∪_⟪1, s \ s'⟫ hv1)) ->
+  HH ∗ H₂ ==> (LGTM.wp [sht_prog] (fun hv1 => LGTM.wp [sht_lang2] fun hv2 => Q (hv2 ∪_⟪1, s'⟫ hv1))) ->
+  HH ∗ H₁ ∗ H₂ ==> LGTM.wp [sht_prog] (fun hv1 => LGTM.wp [sht_lang1] fun hv2 => LGTM.wp [sht_lang2] fun hv3 => Q (hv3 ∪_⟪1, s'⟫ (hv2 ∪_⟪1, s \ s'⟫ hv1)) ) := by
+  move=>prog lang subst disj h1 h2
+  unfold LGTM.wp at h1 h2
+  sorry
+
+
+lemma weird_grmdisj_lemma' (s' s : Set (α × β)) (sht_prog sht_lang : LGTM.SHT) :
   sht_prog.s = ⟪0, s''⟫ ->
   sht_lang.s = ⟪ 1, s⟫ ->
   s' ⊆ s -> Disjoint sht_prog.s sht_lang.s ->
   -- H₃ = HH  (H₁ ∗ H₂) ->
-  HH2 ==> LGTM.wp [sht_prog, ⟨⟪ 1, s \ s'⟫, sht_lang.ht ⟩ ] (fun _ h => ∀ ll ∈ s \ s', ∃ pp, pp ∈ s'' ∧ h ⟨1, ll ⟩= h ⟨0, pp⟩) ->
-  HH1 ==> LGTM.wp [sht_prog, ⟨⟪ 1, s'⟫, sht_lang.ht ⟩ ] (fun _ h => ∀ ll ∈ s', ∃ pp,  pp ∈ s'' ∧ h ⟨1, ll ⟩= h ⟨0, pp⟩) ->
-  HH1 + HH2 ==> LGTM.wp [sht_prog, sht_lang]  (fun v h => ∀ ll ∈ s, ∃ pp, pp ∈ s'' ∧ h ⟨1, ll ⟩= h ⟨0, pp⟩) := by
+  HH ∗ H₁ ==> LGTM.wp [sht_prog, ⟨⟪ 1, s \ s'⟫, sht_lang.ht ⟩ ] (fun _ h => ∀ ll ∈ s \ s', ∃ pp, pp ∈ s'' ∧ h ⟨1, ll ⟩= h ⟨0, pp⟩) ->
+  HH ∗ H₂ ==> LGTM.wp [sht_prog, ⟨⟪ 1, s'⟫, sht_lang.ht ⟩ ] (fun _ h => ∀ ll ∈ s', ∃ pp,  pp ∈ s'' ∧ h ⟨1, ll ⟩= h ⟨0, pp⟩) ->
+  HH ∗ H₁ ∗ H₂ ==> LGTM.wp [sht_prog, sht_lang]  (fun v h => ∀ ll ∈ s, ∃ pp, pp ∈ s'' ∧ h ⟨1, ll ⟩= h ⟨0, pp⟩) := by
   sorry
 
 #check hhand
@@ -762,6 +887,63 @@ lemma weird_payload_lemma (s₁ s₂ : Set (α ⊕ β)) (pr : β) (sht_prog sht_
   move=> up
   simp_all
   use pr
+
+lemma weird_lang_lemma' (s₁ s₂ : Set (trm × β)) (sht_prog sht_lang : LGTM.SHT) :
+  sht_prog.s = ⟪0, s₁⟫ ->
+  sht_lang.s = ⟪ 1, s₂⟫ ->
+  Disjoint sht_prog.s sht_lang.s ->
+  s₂ = {(tl,dp)} ->
+  H ==> LGTM.wp [sht_prog, sht_lang] (fun _ h => ∃ pp ∈ s₁,h ⟨1, (tl,dp) ⟩ = h ⟨0, pp⟩) ->
+  H ==> LGTM.wp [sht_prog, sht_lang] (fun _ h => ∀ ll ∈ s₂, ∃ pp ∈ s₁, h ⟨1, ll ⟩ = h ⟨0,pp⟩) := by
+  move=> prog lang disj set_eq
+  apply weird_post_conseq
+  unfold hqimpl hhimpl
+  intro hv hh
+  simp_all
+
+
+lemma weird_payload_lemma' (s₁ s₂ : Set (α × β)) (sht_prog sht_lang : LGTM.SHT) :
+  sht_prog.s = ⟪0, s₁⟫ ->
+  sht_lang.s = ⟪ 1, s₂⟫ ->
+  Disjoint sht_prog.s sht_lang.s ->
+  pr ∈ s₁ ->
+  H ==> LGTM.wp [sht_prog, sht_lang] (fun _ h => h ⟨1, pl ⟩= h ⟨0, pr⟩) ->
+  H ==> LGTM.wp [sht_prog, sht_lang] (fun _ h => ∃ pp ∈ s₁, h ⟨1, pl ⟩ = h ⟨0, pp⟩):= by
+  move=> prog lang disj set_in
+  apply weird_post_conseq
+  unfold hqimpl hhimpl
+  intro hv hh
+  move=> up
+  use pr
+
+lemma weird_payload_lemma2' (s₁ s₂ : Set (α × β)) (sht_prog sht_lang : LGTM.SHT) :
+  sht_prog.s = ⟪0, s₁⟫ ->
+  sht_lang.s = ⟪ 1, s₂⟫ ->
+  Disjoint sht_prog.s sht_lang.s ->
+  pr ∈ s₁ ->
+  H ==> LGTM.wp [sht_prog, sht_lang] (fun _ h => ∀ ll ∈ s₂, h ⟨1, ll ⟩= h ⟨0, pr⟩) ->
+  H ==> LGTM.wp [sht_prog, sht_lang] (fun _ h => ∀ ll ∈ s₂, ∃ pp ∈ s₁, h ⟨1, ll ⟩ = h ⟨0, pp⟩):= by
+  move=> prog lang disj set_in
+  apply weird_post_conseq
+  unfold hqimpl hhimpl
+  aesop
+
+lemma weird_payload_focus_lemma' (s₁ s₂ : Set (α × β)) (sht_prog sht_lang : LGTM.SHT) :
+  sht_prog.s = ⟪0, s₁⟫ ->
+  sht_lang.s = ⟪ 1, s₂⟫ ->
+  Disjoint sht_prog.s sht_lang.s ->
+  pr ∈ s₁ ->
+  H ==> LGTM.wp [{s:= ⟪0,{pr}⟫, ht:= sht_lang.ht}, sht_lang] (fun _ h => ∀ ll ∈ s₂, h ⟨1, ll ⟩= h ⟨0, pr⟩) ->
+  H ==> LGTM.wp [sht_prog, sht_lang] (fun _ h => ∀ ll ∈ s₂, ∃ pp ∈ s₁, h ⟨1, ll⟩ = h ⟨0, pp⟩):= by
+  move=> prog lang disj set_in
+  sorry
+
+lemma weird_fix_lang (t : trm):
+  H ==> LGTM.wp [sht_prog, { s := ⟪l, {(t, p)}⟫, ht := fun l => t }] Q =
+  H ==> LGTM.wp [sht_prog, { s := ⟪l, {(t, p)}⟫, ht := fun lang => lang.val.1 }] Q := by
+  congr
+  apply LGTM.wp_sht_eq
+  simp_all
 
 lemma weird_seqleft_lemma (s₁ s₂ : Set (α ⊕ β)):
   True := by
